iris/ProofKexecB3.v
@@ -1066,7 +1066,7 @@ Section KexecB3Body.
                            Hivalid & Hload & #Hity & Hfrz & Hkeep & Hru)".
     iDestruct (kxc_load_peel with "Hload") as
       (datl) "(%Hiok & %Hrl & %Hdok & %Hddix & %Hdoc & %Hduq & Hdlk & Hdiat & Hmeta
-               & Hmap & Hblocks & Hdview & Hfview & Htop)".
+               & Hmap & Hblocks & Htop)".
     pose proof Hiok as Hiok'.
     destruct Hiok' as (Hbmwf & Hbmcov & Hdaddr & Hdty & Hszb & Hholes & Hsized).
     iDestruct (proc_priv_bare_acc gf (proc_addr jp) pidv U with "Hpriv")
@@ -1108,7 +1108,7 @@ Section KexecB3Body.
     iDestruct ("Hpvbk" with "Hppid") as "Hpriv".
     iDestruct (kxc_load_seal kf inumf dnf bmf datl
                  Hiok Hrl Hdok Hddix Hdoc Hduq
-                 with "Hdlk Hdiat Hmeta Hmap Hblocks Hdview Hfview Htop") as "Hload".
+                 with "Hdlk Hdiat Hmeta Hmap Hblocks Htop") as "Hload".
     iDestruct (A.kxa_bs3_join with "Hbs1 Hbs2") as "Hbs".
     iDestruct (kxc_open_intro pidv kf qf sf gyf
                  inumf dnf bmf gilf gislf
